src/contracting-refinement/StorageType.v
@@ -1,0 +1,126 @@
+Require Import Memx Predx.
+
+Module Plain.
+Record ResourceSet := {
+    id : Type;
+    resource : Type;
+    id_eq : forall (i i': id), {i=i'}+{i<>i'};
+    resource_map := @mem id id_eq resource;
+    prog : Type -> Type;
+    exec : forall T, resource_map -> prog T -> resource_map -> T -> Prop;
+}.
+
+Record contracting_refinement (High Low : ResourceSet):= {
+    refine_resource: (id High) -> (resource High) -> (resource_map Low);
+    refine_prog : forall T T', (prog High T) -> (prog Low T');
+    refine_ret : forall T T', (prog High T) -> T -> T';
+
+    refine_resource_disjoint :
+      forall hid1 hid2,
+          hid1 <> hid2 ->
+          forall hr1 hr2,
+            @mem_disjoint _ (id_eq Low) _ (refine_resource hid1 hr1) (refine_resource hid2 hr2);
+    
+    refines_to (hm: resource_map High) (lm: resource_map Low) :=
+      (forall hid hr,
+          hm hid = Some hr ->
+          exists m, lm = mem_union m (refine_resource hid hr));
+    
+    refinement_valid:
+      forall T T' (p: prog High T) hm hm' r lm,
+        (exec High) T hm p hm' r ->
+        refines_to hm lm ->
+        exists lm',
+          (exec Low) T' lm (refine_prog T T' p) lm' (refine_ret T T' p r) /\
+          refines_to hm' lm'
+  }.
+End Plain.
+
+Module Owned.
+
+Record OwnedResourceSet := {
+    id : Type;
+    resource : Type;
+    id_eq : forall (i i': id), {i=i'}+{i<>i'};
+    owner : Type;
+    
+    resource_map := @mem id id_eq resource;
+    acl := owner -> id -> Prop;
+
+    equivalent_for: owner -> resource_map -> resource_map -> Prop;
+    
+    prog : Type -> Type;
+    exec : forall T, owner -> acl -> resource_map -> prog T -> acl -> resource_map -> T -> Prop;
+}.
+
+Record single_owner_contracting_refinement (High Low : OwnedResourceSet):=
+  {
+    refine_to_map: id High -> resource High -> resource_map Low;
+    refine_prog : forall T T', (prog High) T -> (prog Low) T';
+    refine_owner : owner High -> owner Low;
+    refine_ret : forall T T', (prog High) T -> T -> T';
+
+    refine_resource_disjoint :
+      forall hid1 hid2,
+          hid1 <> hid2 ->
+          forall hr1 hr2,
+            @mem_disjoint _ (id_eq Low) _ (refine_to_map hid1 hr1) (refine_to_map hid2 hr2);
+
+    acl_refines_to (hacl: acl High) (lacl: acl Low):=
+      forall hid ho hr lid,
+        hacl ho hid ->
+        (refine_to_map hid hr) lid <> None ->
+        lacl (refine_owner ho) lid;
+    
+    map_refines_to (hm: resource_map High) (lm: resource_map Low) :=
+      forall hid hr,
+          hm hid = Some hr ->
+          (exists m, lm = mem_union m (refine_to_map hid hr));
+
+    refinement_preserves_equivalence:
+      forall o hm1 hm2 lm1 lm2,
+        equivalent_for High o hm1 hm2 ->
+        map_refines_to hm1 lm1 ->
+        map_refines_to hm2 lm2 ->
+        equivalent_for Low (refine_owner o) lm1 lm2;
+    
+    refinement_valid:
+      forall T T' o (p: prog High T) hm hm' hacl lacl hacl' r lm,
+        (exec High) T o hacl hm p hacl' hm' r ->
+        map_refines_to hm lm ->
+        acl_refines_to hacl lacl ->
+        exists lacl' lm',
+          (exec Low) T' (refine_owner o) lacl lm (refine_prog T T' p) lacl' lm' (refine_ret T T' p r) /\
+          map_refines_to hm' lm' /\
+          acl_refines_to hacl' lacl'
+  }.
+
+Definition ret_noninterference {T} (layer: OwnedResourceSet) (p: (prog layer) T) :=
+  forall o acl acl' rm1 rm2 rm1' r,
+    (exec layer) _ o acl rm1 p acl' rm1' r ->
+    equivalent_for layer o rm1 rm2 ->
+    (exists rm2',
+      exec layer _ o acl rm2 p acl' rm2' r /\
+      equivalent_for layer o rm1' rm2').
+
+Theorem ret_noninterference_transfer:
+  forall High Low (refinement : single_owner_contracting_refinement High Low) T T' (p: prog High T),
+    ret_noninterference Low ((refine_prog _ _ refinement) T T' p) ->
+    (forall hm, exists lm, map_refines_to _ _ refinement hm lm) ->
+    (forall hacl, exists lacl, acl_refines_to _ _ refinement hacl lacl) ->
+    ret_noninterference High p.
+Proof.
+  unfold ret_noninterference; intros.
+  destruct refinement; simpl in *.
+  specialize (H0 rm1); destruct H0.
+  specialize (H1 acl0); destruct H1.
+  unfold map_refines_to, acl_refines_to in *; simpl in *.
+  
+  specialize refinement_valid0 with (1:= H2)(2:= H0)(3:= H1).
+  specialize (refinement_valid0 T').
+  destruct refinement_valid0.
+  destruct H4.
+  destruct H4.
+  destruct H5.
+Abort.
+End Owned.
